Trying to use equations to define regularity

syntax.sig
@@ -7,6 +7,8 @@ TmApp : Tm -> Tm -> Tm
 
 TyAbs : (bind Ty in Ty) -> Ty
 TyApp : Ty -> Ty -> Ty
+TyForall : Ki -> (bind Ty in Ty) -> Ty
+TyFun : Ty -> Ty -> Ty
 
 Star : Ki
 Arr : Ki -> Ki -> Ki
