theories/typing.v
@@ -5,114 +5,89 @@ Definition TyBasis := list Ki.
 Definition lookup {T} n (Δ : list T) :=
   nth_error Δ n.
 
-Inductive Lookup {T} : nat -> list T -> T -> Prop :=
+Inductive Lookup {T} : nat -> list T -> T -> Type :=
 | Here A Γ : Lookup 0 (A :: Γ) A
 | There n Γ A B : Lookup n Γ A ->
                      Lookup (S n) (cons B Γ) A.
 
-Lemma LookupIff {T} n (Γ : list T) A : Lookup n Γ A <-> lookup n Γ = Some A.
-Proof.
-  split.
-  - elim; hauto lq:on.
-  - elim : n Γ A; hauto q:on inv:list ctrs:Lookup.
-Qed.
+(* Lemma LookupIff {T} n (Γ : list T) A : Lookup n Γ A <-> lookup n Γ = Some A. *)
+(* Proof. *)
+(*   split. *)
+(*   - elim; hauto lq:on. *)
+(*   - elim : n Γ A; hauto q:on inv:list ctrs:Lookup. *)
+(* Qed. *)
 
-Inductive TyWt Δ : Ty -> Ki -> Prop :=
+Inductive TyWt Δ : Ty -> Ki -> Type :=
 | TyT_Var i k :
   Lookup i Δ k ->
   TyWt Δ (VarTy i) k
 
 | TyT_Abs A k0 k1 :
   TyWt (k0 :: Δ) A k1 ->
-  TyWt Δ A (Arr k0 k1)
+  TyWt Δ (TyAbs A) (Arr k0 k1)
 
 | TyT_App b a k0 k1 :
   TyWt Δ b (Arr k0 k1) ->
   TyWt Δ a k0 ->
-  TyWt Δ (TyApp b a) k1.
+  TyWt Δ (TyApp b a) k1
+
+| TyT_Fun A B :
+  TyWt Δ A Star ->
+  TyWt Δ B Star ->
+  TyWt Δ (TyFun A B) Star
+
+| TyT_Forall k A :
+  TyWt (k :: Δ) A Star ->
+  TyWt Δ (TyForall k A) Star.
 
 Definition TmBasis := list Ty.
 
-Definition Basis := list Term.
+(* Lemma lookup_functional {U} n (Γ : list U) A B : Lookup n Γ A -> Lookup n Γ B -> A = B. *)
+(* Proof. rewrite !LookupIff. congruence. Qed. *)
 
-Fixpoint lookup n (Γ : Basis) :=
-  match n, Γ with
-  | O, (cons A  _) => Some (ren_Term S A)
-  | S n, (cons _ Γ) => match lookup n Γ with
-                       | None => None
-                       | Some A => Some (ren_Term S A)
-                       end
-  | _ , _ => None
+Derive Inversion lookup_inv with (forall {U} i (Γ : list U) A, Lookup i Γ A) Sort Prop.
+
+Definition BasisWf Δ Γ := forall i A, Lookup i Γ A -> TyWt Δ A Star.
+
+Fixpoint up_Basis Γ :=
+  match Γ with
+  | nil => nil
+  | A :: Γ => ren_Ty S A :: up_Basis Γ
   end.
 
-Inductive Lookup : nat -> Basis -> Term -> Prop :=
-| Here A Γ : Lookup 0 (A :: Γ) (ren_Term S A)
-| There n Γ A B : Lookup n Γ A ->
-                     Lookup (S n) (cons B Γ) (ren_Term S A).
-
-Lemma LookupIff n Γ A : Lookup n Γ A <-> lookup n Γ = Some A.
-Proof.
-  split.
-  - elim; hauto lq:on.
-  - elim : n Γ A; hauto q:on inv:list ctrs:Lookup.
-Qed.
-
-Lemma lookup_functional n Γ A B : Lookup n Γ A -> Lookup n Γ B -> A = B.
-Proof. rewrite !LookupIff. congruence. Qed.
-
-Derive Inversion lookup_inv with (forall i Γ A, Lookup i Γ A) Sort Prop.
-
-Inductive Wt : Basis -> Term -> Term -> Prop :=
-| T_Var Γ i A :
-  ⊢ Γ ->
+Inductive Wt Δ Γ : Tm -> Ty -> Type :=
+| T_Var i A :
+  BasisWf Δ Γ ->
   Lookup i Γ A ->
   (* ----------- *)
-  Γ ⊢ VarTm i ∈ A
+  Wt Δ Γ (VarTm i) A
 
-| T_Star Γ :
-  ⊢ Γ ->
-  (* --------- *)
-  Γ ⊢ ISort Star ∈ ISort Kind
-
-| T_Abs Γ A s1 a B s2 :
-  Γ ⊢ A ∈ ISort s1 ->
-  A :: Γ ⊢ a ∈ B ->
-  A :: Γ ⊢ B ∈ ISort s2 ->
+| T_Abs A a B :
+  TyWt Δ A Star ->
+  Wt Δ (A :: Γ) a B ->
   (* -------------------- *)
-  Γ ⊢ Abs A a ∈ Pi A B
+  Wt Δ Γ (TmAbs a) (TyFun A B)
 
-| T_App Γ a b A B :
-  Γ ⊢ a ∈ A ->
-  Γ ⊢ b ∈ Pi A B ->
+| T_App a b A B :
+  Wt Δ Γ a A ->
+  Wt Δ Γ b (TyFun A B) ->
   (* --------------- *)
-  Γ ⊢ App b a ∈ B[a…]
+  Wt Δ Γ (TmApp b a) B
 
-| T_Pi Γ A s1 B s2 :
-  Γ ⊢ A ∈ ISort s1 ->
-  A :: Γ ⊢ B ∈ ISort s2 ->
-  (* -------------------- *)
-  Γ ⊢ Pi A B ∈ ISort s2
+| T_Forall k a A :
+  Wt (k :: Δ) (up_Basis Γ) a A ->
+  (* --------------------------- *)
+  Wt Δ Γ a (TyForall k A)
 
-| T_Conv Γ a A B s :
-  Γ ⊢ a ∈ A ->
-  Γ ⊢ B ∈ ISort s ->
-  A ⇔ B ->
+| T_Inst k a A B :
+  TyWt Δ B k ->
+  Wt Δ Γ a (TyForall k A) ->
+  (* ------------------------ *)
+  Wt Δ Γ a (subst_Ty (B…) A)
+
+| T_Conv a A B :
+  Wt Δ Γ a A ->
+  TyWt Δ B Star ->
+  ICoherent A B ->
   (* ------------ *)
-  Γ ⊢ a ∈ B
-
-with Wf : Basis -> Prop :=
-| Wf_Nil :
-  (* --- *)
-  ⊢ nil
-
-| Wf_Cons Γ A s :
-  ⊢ Γ ->
-  Γ ⊢ A ∈ ISort s ->
-  (* ----------- *)
-  ⊢ A :: Γ
-
-where "Γ ⊢ a ∈ A" := (Wt Γ a A) and "⊢ Γ" := (Wf Γ).
-
-Scheme Wt_ind_2 := Induction for Wt Sort Prop
-    with Wf_ind_2 := Induction for Wf Sort Prop.
-Combined Scheme Wt_multind from Wt_ind_2, Wf_ind_2.
+  Wt Δ Γ a B.
